*** empty log message ***

doc-src/TutorialI/Advanced/WFrec.thy
@@ -26,11 +26,14 @@ recursion}\indexbold{recursion!wellfounded}\index{wellfounded
 recursion|see{recursion, wellfounded}}.  A relation $<$ is
 \bfindex{wellfounded} if it has no infinite descending chain $\cdots <
 a@2 < a@1 < a@0$. Clearly, a function definition is total iff the set
-of all pairs $(r,l)$, where $l$ is the argument on the left-hand side of an equation
-and $r$ the argument of some recursive call on the corresponding
-right-hand side, induces a wellfounded relation.  For a systematic
-account of termination proofs via wellfounded relations see, for
-example, \cite{Baader-Nipkow}.
+of all pairs $(r,l)$, where $l$ is the argument on the left-hand side
+of an equation and $r$ the argument of some recursive call on the
+corresponding right-hand side, induces a wellfounded relation.  For a
+systematic account of termination proofs via wellfounded relations
+see, for example, \cite{Baader-Nipkow}. The HOL library formalizes
+some of the theory of wellfounded relations. For example
+@{prop"wf r"}\index{*wf|bold} means that relation @{term[show_types]"r::('a*'a)set"} is
+wellfounded.
 
 Each \isacommand{recdef} definition should be accompanied (after the
 name of the function) by a wellfounded relation on the argument type
@@ -40,7 +43,68 @@ and it has been proved that @{term"measure f"} is always wellfounded.
 
 In addition to @{term measure}, the library provides
 a number of further constructions for obtaining wellfounded relations.
-
-wf proof auto if stndard constructions.
+Above we have already met @{text"<*lex*>"} of type
+@{typ[display,source]"('a \<times> 'a)set \<Rightarrow> ('b \<times> 'b)set \<Rightarrow> (('a \<times> 'b) \<times> ('a \<times> 'b))set"}
+Of course the lexicographic product can also be interated, as in the following
+function definition:
 *}
+
+consts contrived :: "nat \<times> nat \<times> nat \<Rightarrow> nat"
+recdef contrived
+  "measure(\<lambda>i. i) <*lex*> measure(\<lambda>j. j) <*lex*> measure(\<lambda>k. k)"
+"contrived(i,j,Suc k) = contrived(i,j,k)"
+"contrived(i,Suc j,0) = contrived(i,j,j)"
+"contrived(Suc i,0,0) = contrived(i,i,i)"
+"contrived(0,0,0)     = 0"
+
+text{*
+Lexicographic products of measure functions already go a long way. A
+further useful construction is the embedding of some type in an
+existing wellfounded relation via the inverse image of a function:
+@{thm[display,show_types]inv_image_def[no_vars]}
+\begin{sloppypar}
+\noindent
+For example, @{term measure} is actually defined as @{term"inv_mage less_than"}, where
+@{term less_than} of type @{typ"(nat \<times> nat)set"} is the less-than relation on type @{typ nat}
+(as opposed to @{term"op <"}, which is of type @{typ"nat \<Rightarrow> nat \<Rightarrow> bool"}).
+\end{sloppypar}
+
+%Finally there is also {finite_psubset} the proper subset relation on finite sets
+
+All the above constructions are known to \isacommand{recdef}. Thus you
+will never have to prove wellfoundedness of any relation composed
+solely of these building blocks. But of course the proof of
+termination of your function definition, i.e.\ that the arguments
+decrease with every recursive call, may still require you to provide
+additional lemmas.
+
+It is also possible to use your own wellfounded relations with \isacommand{recdef}.
+Here is a simplistic example:
+*}
+
+consts f :: "nat \<Rightarrow> nat"
+recdef f "id(less_than)"
+"f 0 = 0"
+"f (Suc n) = f n"
+
+text{*
+Since \isacommand{recdef} is not prepared for @{term id}, the identity
+function, this leads to the complaint that it could not prove
+@{prop"wf (id less_than)"}, the wellfoundedness of @{term"id
+less_than"}. We should first have proved that @{term id} preserves wellfoundedness
+*}
+
+lemma wf_id: "wf r \<Longrightarrow> wf(id r)"
+by simp;
+
+text{*\noindent
+and should have added the following hint to our above definition:
+*}
+(*<*)
+consts g :: "nat \<Rightarrow> nat"
+recdef g "id(less_than)"
+"g 0 = 0"
+"g (Suc n) = g n"
+(*>*)
+(hints recdef_wf add: wf_id)
 (*<*)end(*>*)
